src/computational_monads/simulation_semantics/is_stateless.lean
@@ -1,0 +1,77 @@
+/-
+Copyright (c) 2023 Devon Tuma. All rights reserved.
+Released under Apache 2.0 license as described in the file LICENSE.
+Authors: Devon Tuma
+-/
+import computational_monads.simulation_semantics.is_tracking
+
+/-!
+# Tracking Simulation Oracles
+
+This file defines a typeclass `sim_oracle.is_stateless` for oracles in which there is no
+meaningful internal state, represented by the state type being `subsingleton`.
+This is a special case of `sim_oracle.is_tracking`, see `is_stateless.is_tracking`.
+This allows for a number of very general lemmas that simplify the process of working
+with simulated computations, by automatically removing states.
+-/
+
+variables {α β γ : Type} {spec spec' spec'' : oracle_spec} {S S' : Type}
+
+open_locale big_operators ennreal
+open oracle_comp oracle_spec
+
+namespace sim_oracle
+
+/-- Class to represent oracles that make no use of their internal state.
+This class is introduced rather than using a `subsingleton` hypothesis directly
+in order to create a unified `is_tracking` instance based on this fact.
+This also allows typeclass resolution to work "backwords", in that subsingleton instances don't
+have to be defined on the type parameter `S` explicitly, but on the actual oracle instead. -/
+class is_stateless (so : sim_oracle spec spec' S) :=
+(state_subsingleton : subsingleton S)
+
+variables (so : sim_oracle spec spec' S) (i : spec.ι)
+  (t t' : spec.domain i) (s s' : S) (u u' : spec.range i)
+
+/-- Specialize `subsingleton.elim` to simplify the state to the default oracle state.
+Usefull for giving a unified convergence point for state values. -/
+lemma state_elim [hso : so.is_stateless] (s : S) : s = so.default_state :=
+@subsingleton.elim S hso.state_subsingleton s so.default_state
+
+instance is_stateless.is_tracking [hso : so.is_stateless] : so.is_tracking :=
+{
+  query_f := λ i t, prod.fst <$> so i (t, so.default_state),
+  state_f := λ s i t u, so.default_state,
+  apply_equiv_state_f_map_query_f :=
+    begin
+      refine λ i t s, trans ((eval_dist_map_id $ (so i (t, s))).symm.trans
+        (map_equiv_congr (λ x, _) (by rw so.state_elim s))) (eval_dist_map_comp' _ _ _).symm,
+      simp only [prod.eq_iff_fst_eq_snd_eq, so.state_elim x.2, id.def, eq_self_iff_true, and_self]
+    end
+}
+
+namespace is_stateless
+
+variable [is_stateless so]
+
+@[simp] lemma answer_query.def : so.answer_query =
+  λ i t, prod.fst <$> so i (t, so.default_state) := rfl
+
+@[simp] lemma update_state.def : so.update_state =
+  λ s i t u, so.default_state := rfl
+
+section support
+
+lemma support_apply' : (so i (t, s)).support =
+  ((λ u, (u, so.default_state)) <$> so.answer_query i t).support :=
+by simp only [is_tracking.support_apply', update_state.def]
+
+lemma support_apply : (so i (t, s)).support =
+  (λ u, (u, so.default_state)) '' (so.answer_query i t).support :=
+by rw [support_apply', support_map]
+
+end support
+
+end is_stateless
+
+end sim_oracle
